stubbing out invariants and dispatch

snglswch/lucid_base_rec.dfy
@@ -2,26 +2,41 @@
 // Phrasing it as a recursive method
 // made it a _lot_ easier to reason about
 
-abstract module Interp {
+abstract module LucidBase {
+    type bits = x : int | 0 <= x < 256                 // number must match
+    const T : nat := 256
     type Event (==)
-    datatype LocEvent = LocEvent(e : Event, time : nat)
-    type State = seq<int>
-    class Prog {
+    datatype LocEvent = LocEvent(e : Event, time : bits, natTime : nat)
+    class State {
+        constructor () 
+            ensures fresh(this)
+        { }
+    }
+    class Handlers { // maybe should be "prog" or something. Not just handlers, really.
+
+
         // state and event queue are mutable for user-facing abstractions
         var state : State
         var queue : seq<LocEvent> // event * timestamp
+        var natTime : nat
+        var lastNatTime : nat
 
         /***   user-defined predicates   ***/
         // an invariant over the last event that was processed, the current event, and the remaining events
-        ghost predicate user_event_invariant(s : State, cur_ev : LocEvent, ev_queue : seq<LocEvent>)
+        ghost predicate inter_event_invariant(s : State, cur_ev : LocEvent, ev_queue : seq<LocEvent>, lastNatTime : nat)
         // a predicate that must hold over the entire event queue before and after 
         // dispatch, that defines the pairs of events that we may see
-        ghost predicate valid_next_event(cur_ev : LocEvent, next_ev : LocEvent)
-
+        ghost predicate valid_next_event(cur : LocEvent, next : LocEvent)
 
         ghost predicate valid_event_queue(ev_queue : seq<LocEvent>)
         {
-            forall i | 1 <= i < |ev_queue| :: valid_next_event(ev_queue[i-1], ev_queue[i])
+            (forall i | 1 <= i < |ev_queue| :: (
+                valid_next_event(ev_queue[i-1], ev_queue[i])
+                && ev_queue[i-1].natTime <= ev_queue[i].natTime)
+            )
+            && 
+            (forall i | 0 <= i < |ev_queue| - 1 :: 
+                ev_queue[i].time == (ev_queue[i].natTime % T))
         }
 
         lemma valid_event_queue_implies_valid_head(ev_queue : seq<LocEvent>)
@@ -39,8 +54,10 @@ abstract module Interp {
         method ProcessEvent(i : nat, eq : seq<LocEvent>) returns (j : nat)
             requires |eq| > 0
             requires valid_event_queue(eq)
-            requires user_event_invariant(this.state, eq[0], eq[1..])
-            modifies this`queue, this`state
+            requires inter_event_invariant(this.state, eq[0], eq[1..], lastNatTime)
+            requires lastNatTime <= eq[0].natTime
+            requires this.natTime == eq[0].natTime
+            modifies this`queue, this`state, this`lastNatTime, this`natTime
         {
             if (i <= 0) {
                 j := 0;
@@ -49,7 +66,7 @@ abstract module Interp {
                 var ev_head := eq[0];
                 var eq_tail := eq[1..];
                 this.queue := eq_tail;
-                assert user_event_invariant(this.state, ev_head, queue);                
+                assert inter_event_invariant(this.state, ev_head, queue, lastNatTime);                
                 Dispatch(ev_head);
                 // if the queue is now empty, we are done
                 if (queue == []) {
@@ -73,16 +90,19 @@ abstract module Interp {
                     valid_event_queue_implies_valid_tail([ev_head]+queue);
                     // assert valid_event_queue(queue);
                     // assert valid_event_queue(queue[1..]);
-                    // so now we can just recurse!
+                    // so now we can just update the times and recurse!
+                    this.lastNatTime := natTime;
+                    this.natTime := queue[0].natTime;
                     j := ProcessEvent(i-1, this.queue);
                 }
             }
         }
 
+
         method Dispatch(cur_ev : LocEvent)
             modifies this`state, this`queue
             // at the start of dispatch, the user event invariant must hold for the current event
-            requires user_event_invariant(this.state, cur_ev, this.queue)
+            requires inter_event_invariant(this.state, cur_ev, this.queue, this.lastNatTime)
             // and the event must be part of a valid sequence of events
             requires valid_event_queue([cur_ev] + this.queue)
             // after processing, if the queue has more items in it to process, 
@@ -95,10 +115,14 @@ abstract module Interp {
             //   the current state and the remaining event queue
             ensures (
                 |queue| > 0 ==> 
-                    (forall ev : LocEvent | valid_next_event(cur_ev, ev) :: user_event_invariant(this.state, ev, this.queue[1..]))
+                    (forall ev : LocEvent | valid_next_event(cur_ev, ev) :: inter_event_invariant(this.state, ev, this.queue[1..], cur_ev.natTime))
             )
             // and the event must still be part of a valid sequence of events
             ensures  valid_event_queue([cur_ev] + this.queue)
+
+
+
+
     }
 
 }
